Verify all store operations except [store_restore].

theories/store.v
@@ -7,6 +7,8 @@ From iris.base_logic Require Import
 
 From zebre Require Import
   prelude.
+From zebre.iris.base_logic Require Import
+  lib.mono_map_.
 From zebre.language Require Import
   notations
   diaframe.
@@ -15,6 +17,11 @@ From zebre.std Require Import
   lst.
 From zebre Require Import
   options.
+
+Implicit Types l r node cnode base root dst : loc.
+Implicit Types nodes : list loc.
+Implicit Types v t s : val.
+Implicit Types σ : gmap loc val.
 
 #[local] Notation "'gen'" := (
   in_type "t" 0
@@ -134,30 +141,595 @@ Definition store_restore : val :=
       end
     ).
 
-Implicit Types l r node cnode base root dst : loc.
-Implicit Types nodes : list loc.
-Implicit Types v t s : val.
-Implicit Types σ : gmap loc val.
+Module raw.
+  #[local] Definition generation :=
+    nat.
+  Implicit Types g : generation.
 
-#[local] Definition generation :=
-  nat.
-Implicit Types g : generation.
+  #[local] Definition store :=
+    gmap loc (generation * val).
+  Implicit Types ς : store.
+  Implicit Types data : generation * val.
 
-#[local] Definition store :=
-  gmap loc (generation * val).
-Implicit Types ς : store.
-Implicit Types data : generation * val.
+  #[local] Definition descriptor : Set :=
+    generation * store.
+  Implicit Types descr base_descr : descriptor.
 
-#[local] Definition descriptor : Set :=
-  generation * store.
-Implicit Types descr base_descr : descriptor.
+  Class StoreG Σ `{zebre_G : !ZebreG Σ} := {
+    #[local] store_G_nodes_G :: ghost_mapG Σ loc descriptor ;
+  }.
+
+  Definition store_Σ := #[
+    ghost_mapΣ loc descriptor
+  ].
+  #[global] Instance subG_store_Σ Σ `{zebre_G : !ZebreG Σ} :
+    subG store_Σ Σ →
+    StoreG Σ.
+  Proof.
+    solve_inG.
+  Qed.
+
+  Section store_G.
+    Context `{store_G : StoreG Σ}.
+
+    #[local] Definition store_on σ0 ς :=
+      ς ∪ (pair 0 <$> σ0).
+    #[local] Definition store_generation g ς :=
+      map_Forall (λ r data, data.1 ≤ g) ς.
+
+    #[local] Definition descriptor_wf σ0 descr :=
+      dom descr.2 ⊆ dom σ0 ∧
+      store_generation descr.1 descr.2.
+
+    #[local] Definition delta : Set :=
+      loc * (generation * val).
+    Implicit Types δ : delta.
+    Implicit Types δs : list delta.
+
+    #[local] Definition deltas_apply δs ς :=
+      list_to_map δs ∪ ς.
+    #[local] Fixpoint deltas_chain node nodes δs dst : iProp Σ :=
+      match nodes, δs with
+      | [], [] =>
+          ⌜node = dst⌝
+      | node' :: nodes, δ :: δs =>
+          node ↦ ’Diff{ #δ.1, #δ.2.1, δ.2.2, #node' } ∗
+          deltas_chain node' nodes δs dst
+      | _, _ =>
+          False
+      end.
+
+    #[local] Definition cnodes_auth γ cnodes :=
+      ghost_map_auth γ 1 cnodes.
+    #[local] Definition cnodes_elem γ cnode descr :=
+      ghost_map_elem γ cnode DfracDiscarded descr.
+
+    #[local] Definition cnode_model is_base γ σ0 cnode descr node ς : iProp Σ :=
+      ⌜descriptor_wf σ0 descr⌝ ∗
+      cnodes_elem γ cnode descr ∗
+      ( ∃ nodes δs,
+        ⌜NoDup δs.*1⌝ ∗
+        ⌜ if is_base is Some g then
+            Forall (λ δ, ∃ data, ς !! δ.1 = Some data ∧ data.1 = g) δs
+          else
+            0 < length δs
+        ⌝ ∗
+        ⌜store_on σ0 descr.2 = store_on σ0 $ deltas_apply δs ς⌝ ∗
+        deltas_chain cnode nodes δs node
+      ).
+    Definition store_model t σ0 σ : iProp Σ :=
+      ∃ l γ g root ς,
+      ⌜t = #l⌝ ∗
+      ⌜σ = snd <$> ς⌝ ∗
+      meta l (nroot.@"impl") γ ∗
+      l.[gen] ↦ #g ∗
+      l.[root] ↦ #root ∗
+      root ↦ §Root ∗
+      ( [∗ map] r ↦ data ∈ store_on σ0 ς,
+        r.[ref_gen] ↦ #data.1 ∗
+        r.[ref_value] ↦ data.2
+      ) ∗
+      ⌜descriptor_wf σ0 (g, ς)⌝ ∗
+      if decide (g = 0) then
+        cnodes_auth γ ∅
+      else
+        ∃ cnodes base base_descr,
+        cnodes_auth γ cnodes ∗
+        (* base cnode *)
+        ⌜cnodes !! base = Some base_descr⌝ ∗
+        ⌜base_descr.1 < g⌝ ∗
+        cnode_model (Some g) γ σ0 base base_descr root ς ∗
+        (* other cnodes *)
+        ( [∗ map] cnode ↦ descr ∈ delete base cnodes,
+          ∃ cnode' descr',
+          ⌜cnodes !! cnode' = Some descr'⌝ ∗
+          cnode_model None γ σ0 cnode descr cnode' descr'.2
+        ).
+
+    Definition store_snapshot_model s t σ : iProp Σ :=
+      ∃ l γ g node descr,
+      ⌜t = #l ∧ s = (t, #g, #node)%V⌝ ∗
+      meta l (nroot.@"impl") γ ∗
+      cnodes_elem γ node descr ∗
+      ⌜descr.1 ≤ g⌝.
+
+    #[global] Instance store_model_timeless t σ0 σ :
+      Timeless (store_model t σ0 σ).
+    Proof.
+    Admitted.
+    #[global] Instance store_snapshot_persistent s t σ :
+      Persistent (store_snapshot_model s t σ).
+    Proof.
+      apply _.
+    Qed.
+
+    #[local] Lemma store_on_dom σ0 ς :
+      dom (store_on σ0 ς) = dom σ0 ∪ dom ς.
+    Proof.
+      set_solver.
+    Qed.
+    #[local] Lemma store_on_dom' σ0 ς :
+      dom ς ⊆ dom σ0 →
+      dom (store_on σ0 ς) = dom σ0.
+    Proof.
+      set_solver.
+    Qed.
+    #[local] Lemma store_on_lookup {σ0 ς} r data :
+      store_on σ0 ς !! r = Some data ↔
+          ς !! r = Some data
+        ∨ ς !! r = None ∧
+          data.1 = 0 ∧
+          σ0 !! r = Some data.2.
+    Proof.
+      destruct data as (g, v).
+      rewrite lookup_union_Some_raw lookup_fmap_Some. naive_solver.
+    Qed.
+    #[local] Lemma store_on_lookup' {σ0 ς} r data :
+      ς !! r = Some data →
+      store_on σ0 ς !! r = Some data.
+    Proof.
+      apply lookup_union_Some_l.
+    Qed.
+    #[local] Lemma store_on_insert r data σ0 ς :
+      store_on σ0 (<[r := data]> ς) = <[r := data]> (store_on σ0 ς).
+    Proof.
+      rewrite insert_union_l //.
+    Qed.
+    #[local] Lemma store_on_insert_support r v σ0 ς :
+      σ0 !! r = None →
+      dom ς ⊆ dom σ0 →
+      store_on (<[r := v]> σ0) ς = <[r := (0, v)]> (store_on σ0 ς).
+    Proof.
+      intros Hr%not_elem_of_dom Hς_dom.
+      assert (ς !! r = None).
+      { apply not_elem_of_dom. set_solver. }
+      rewrite insert_union_r // -fmap_insert //.
+    Qed.
+
+    #[local] Lemma deltas_apply_nil ς :
+      deltas_apply [] ς = ς.
+    Proof.
+      rewrite /deltas_apply list_to_map_nil left_id //.
+    Qed.
+    #[local] Lemma deltas_apply_cons δ δs ς :
+      deltas_apply (δ :: δs) ς = <[δ.1 := δ.2]> (deltas_apply δs ς).
+    Proof.
+      destruct δ as (r, data).
+      rewrite /deltas_apply list_to_map_cons insert_union_l //.
+    Qed.
+    #[local] Lemma deltas_apply_singleton δ ς :
+      deltas_apply [δ] ς = <[δ.1 := δ.2]> ς.
+    Proof.
+      rewrite deltas_apply_cons deltas_apply_nil //.
+    Qed.
+    #[local] Lemma deltas_apply_app δs1 δs2 ς :
+      deltas_apply (δs1 ++ δs2) ς = deltas_apply δs1 (deltas_apply δs2 ς).
+    Proof.
+      rewrite /deltas_apply list_to_map_app assoc //.
+    Qed.
+    #[local] Lemma deltas_apply_snoc δs δ ς :
+      deltas_apply (δs ++ [δ]) ς = deltas_apply δs (<[δ.1 := δ.2]> ς).
+    Proof.
+      rewrite deltas_apply_app deltas_apply_singleton //.
+    Qed.
+    #[local] Lemma deltas_apply_snoc' δs r data ς :
+      deltas_apply (δs ++ [(r, data)]) ς = deltas_apply δs (<[r := data]> ς).
+    Proof.
+      apply (deltas_apply_snoc _ (r, data)).
+    Qed.
+    #[local] Lemma deltas_apply_dom δs ς :
+      dom (deltas_apply δs ς) = list_to_set δs.*1 ∪ dom ς.
+    Proof.
+      rewrite dom_union_L. f_equal. apply dom_list_to_map_L.
+    Qed.
+    #[local] Lemma deltas_apply_lookup r data δs ς :
+      NoDup δs.*1 →
+      (r, data) ∈ δs →
+      deltas_apply δs ς !! r = Some data.
+    Proof.
+      intros Hδs_nodup Hδ.
+      apply lookup_union_Some_l, elem_of_list_to_map_1; done.
+    Qed.
+    #[local] Lemma deltas_apply_lookup_ne r δs ς :
+      NoDup δs.*1 →
+      r ∉ δs.*1 →
+      deltas_apply δs ς !! r = ς !! r.
+    Proof.
+      intros Hδs_nodup Hr.
+      apply lookup_union_r, not_elem_of_list_to_map_1. done.
+    Qed.
+    #[local] Lemma deltas_apply_permutation {δs1} δs2 ς :
+      NoDup δs1.*1 →
+      δs1 ≡ₚ δs2 →
+      deltas_apply δs1 ς = deltas_apply δs2 ς.
+    Proof.
+      intros. rewrite /deltas_apply (list_to_map_proper _ δs2) //.
+    Qed.
+
+    #[local] Lemma deltas_chain_nil_inv node nodes dst :
+      deltas_chain node nodes [] dst ⊢
+      ⌜nodes = [] ∧ node = dst⌝.
+    Proof.
+      destruct nodes; iSteps.
+    Qed.
+    #[local] Lemma deltas_chain_cons_inv node nodes δ δs dst :
+      deltas_chain node nodes (δ :: δs) dst ⊢
+        ∃ node' nodes',
+        ⌜nodes = node' :: nodes'⌝ ∗
+        node ↦ ’Diff{ #δ.1, #δ.2.1, δ.2.2, #node' } ∗
+        deltas_chain node' nodes' δs dst.
+    Proof.
+      destruct nodes; iSteps.
+    Qed.
+    #[local] Lemma deltas_chain_snoc {node nodes δs dst} r g v dst' :
+      deltas_chain node nodes δs dst -∗
+      dst ↦ ’Diff{ #r, #g, v, #dst' } -∗
+      deltas_chain node (nodes ++ [dst']) (δs ++ [(r, (g, v))]) dst'.
+    Proof.
+      iInduction nodes as [] "IH" forall (node δs); destruct δs; iSteps.
+    Qed.
+
+    #[local] Definition cnodes_alloc root :
+      ⊢ |==>
+        ∃ γ,
+        cnodes_auth γ ∅.
+    Proof.
+      iMod ghost_map_alloc as "(%γ & Hcnodes_auth & _)".
+      iSteps.
+    Qed.
+    #[local] Lemma cnodes_insert {γ cnodes} cnode descr :
+      cnodes !! cnode = None →
+      cnodes_auth γ cnodes ⊢ |==>
+        cnodes_auth γ (<[cnode := descr]> cnodes) ∗
+        cnodes_elem γ cnode descr.
+    Proof.
+      iIntros "%Hcnodes_lookup Hcnodes_auth".
+      iMod (ghost_map_insert with "Hcnodes_auth") as "($ & Hcnodes_elem)"; first done.
+      iApply (ghost_map_elem_persist with "Hcnodes_elem").
+    Qed.
+
+    Lemma store_model_valid t σ0 σ :
+      store_model t σ0 σ ⊢
+      ⌜dom σ ⊆ dom σ0⌝.
+    Proof.
+      iIntros "(%l & %γ & %g & %root & %ς & -> & -> & #Hmeta & Hl_gen & Hl_root & Hroot & Hς & (%Hς_dom & %Hς_gen) & _)".
+      rewrite dom_fmap //.
+    Qed.
+
+    Lemma store_create_spec :
+      {{{ True }}}
+        store_create ()
+      {{{ t,
+        RET t;
+        (∃ l, ⌜t = #l⌝ ∗ meta_token l (↑nroot.@"user")) ∗
+        store_model t ∅ ∅
+      }}}.
+    Proof.
+      iIntros "%Φ _ HΦ".
+      wp_rec.
+      wp_alloc root as "Hroot".
+      wp_record l as "Hmeta" "(Hl_gen & Hl_root & _)".
+      iMod (cnodes_alloc root) as "(%γ & Hcnodes_auth)".
+      iDestruct (meta_token_difference _ (↑nroot.@"user") with "Hmeta") as "(Hmeta_user & Hmeta)"; first done.
+      iDestruct (meta_token_difference _ (↑nroot.@"impl") with "Hmeta") as "(Hmeta & _)"; first solve_ndisj.
+      iMod (meta_set with "Hmeta") as "Hmeta"; first done.
+      iApply "HΦ".
+      iStep. iExists l, γ, 0, root, ∅. iFrame. rewrite big_sepM_empty. iSteps.
+    Qed.
+
+    Lemma store_ref_spec t σ0 σ v :
+      {{{
+        store_model t σ0 σ
+      }}}
+        store_ref t v
+      {{{ r,
+        RET #r;
+        ⌜σ0 !! r = None⌝ ∗
+        store_model t (<[r := v]> σ0) σ
+      }}}.
+    Proof.
+      iIntros "%Φ (%l & %γ & %g & %root & %ς & -> & -> & #Hmeta & Hl_gen & Hl_root & Hroot & Hς & (%Hς_dom & %Hς_gen) & Hmodel) HΦ".
+      wp_rec. wp_record r as "(Hr_gen & Hr_value & _)".
+      iAssert ⌜σ0 !! r = None⌝%I as %Hr.
+      { rewrite -not_elem_of_dom. iIntros "%Hr".
+        iDestruct (big_sepM_lookup with "Hς") as "(_Hr_gen & _)".
+        { apply lookup_lookup_total_dom. rewrite store_on_dom' //. }
+        iDestruct (pointsto_ne with "Hr_gen _Hr_gen") as %?. done.
+      }
+      iApply "HΦ".
+      iSplitR; first iSteps. iExists l, γ, g, root, ς. iFrame "#∗". iStep 2.
+      iSplitL "Hς Hr_gen Hr_value".
+      { rewrite store_on_insert_support //.
+        iApply (big_sepM_insert_2 with "[Hr_gen Hr_value] Hς").
+        iSteps.
+      }
+      iSplitR. { iPureIntro. split; [set_solver | done]. }
+      case_decide as Hg; first iSteps.
+      iStep 3 as (cnodes base base_descr _ Hbase_gen (Hbase_store_dom & Hbase_store_gen) nodes δs Hδs_nodup Hδs_gen Hδs) "Hcnodes_elem_base Hδs Hcnodes". iSteps.
+      { iPureIntro. set_solver. }
+      { iPureIntro.
+        rewrite !store_on_insert_support //; last congruence.
+        apply (f_equal dom) in Hδs. set_solver.
+      } {
+        iApply (big_sepM_impl with "Hcnodes"). iIntros "!> !> %cnode %descr %Hcnodes_lookup (%cnode' & %descr' & %Hcnodes_lookup' & ((%Hcnode_store_dom & %Hcnode_store_gen) & #Hcnodes_elem_cnode & (%nodes' & %δs' & %Hδs'_nodup & %Hδs'_length & %Hδs' & Hδs')))".
+        iExists cnode', descr'. iSteps; iPureIntro; first set_solver.
+        rewrite !store_on_insert_support //; last congruence.
+        apply (f_equal dom) in Hδs'. set_solver.
+      }
+    Qed.
+
+    Lemma store_get_spec {t σ0 σ r} v :
+      (σ ∪ σ0) !! r = Some v →
+      {{{
+        store_model t σ0 σ
+      }}}
+        store_get t #r
+      {{{
+        RET v;
+        store_model t σ0 σ
+      }}}.
+    Proof.
+      iIntros "%Hσ_lookup %Φ (%l & %γ & %g & %root & %ς & -> & -> & #Hmeta & Hl_gen & Hl_root & Hroot & Hς & (%Hς_dom & %Hς_gen) & Hmodel) HΦ".
+      wp_rec.
+      assert (∃ g_r, store_on σ0 ς !! r = Some (g_r, v)) as (g_r & Hς_lookup).
+      { setoid_rewrite store_on_lookup.
+        apply lookup_union_Some_raw in Hσ_lookup as [Hσ_lookup | (Hσ_lookup & Hσ0_lookup)].
+        - apply lookup_fmap_Some in Hσ_lookup as ((g_r & _v) & ? & Hς_lookup).
+          naive_solver.
+        - rewrite lookup_fmap fmap_None in Hσ_lookup.
+          naive_solver.
+      }
+      iDestruct (big_sepM_lookup_acc with "Hς") as "((Hr_gen & Hr_value) & Hς)"; first done.
+      wp_load.
+      iSteps.
+    Qed.
+
+    Lemma store_set_spec t σ0 σ r v :
+      r ∈ dom σ0 →
+      {{{
+        store_model t σ0 σ
+      }}}
+        store_set t #r v
+      {{{
+        RET ();
+        store_model t σ0 (<[r := v]> σ)
+      }}}.
+    Proof.
+      iIntros "%Hr %Φ (%l & %γ & %g & %root & %ς & -> & -> & #Hmeta & Hl_gen & Hl_root & Hroot & Hς & (%Hς_dom & %Hς_gen) & Hmodel) HΦ".
+      pose proof Hr as (w0 & Hσ0_lookup)%elem_of_dom.
+      wp_rec. wp_load.
+      assert (∃ g_r w, store_on σ0 ς !! r = Some (g_r, w) ∧ g_r ≤ g) as (g_r & w & Hς_lookup & Hg_r).
+      { setoid_rewrite store_on_lookup.
+        destruct (ς !! r) as [(g_r, w) |] eqn:Hς_lookup.
+        - exists g_r, w. split; first naive_solver.
+          opose proof* map_Forall_lookup_1; done.
+        - exists 0, w0. split; first naive_solver. lia.
+      }
+      iDestruct (big_sepM_insert_acc with "Hς") as "((Hr_gen & Hr_value) & Hς)"; first done.
+      wp_load. wp_pures.
+      destruct (decide (g = 0)) as [-> | Hg].
+      - assert (g_r = 0) as -> by lia.
+        rewrite bool_decide_eq_true_2 //. wp_pures.
+        wp_store.
+        iDestruct ("Hς" $! (0, v) with "[$Hr_gen $Hr_value]") as "Hς".
+        iApply "HΦ".
+        iExists l, γ, 0, root, (<[r := (0, v)]> ς). iFrame "#∗". iStep.
+        iSplitR. { rewrite fmap_insert //. }
+        iSplitL. { rewrite insert_union_l //. }
+        iPureIntro. split; first set_solver. apply map_Forall_insert_2; done.
+      - destruct (decide (g = g_r)) as [<- | Hcase].
+        + rewrite bool_decide_eq_true_2 //.
+          wp_store.
+          iDestruct ("Hς" $! (g, v) with "[$Hr_gen $Hr_value]") as "Hς".
+          iApply "HΦ".
+          iExists l, γ, g, root, (<[r := (g, v)]> ς). iFrame "#∗". iStep.
+          iSplitR. { rewrite fmap_insert //. }
+          iSplitL "Hς". { rewrite insert_union_l //. }
+          iSplitR. { iPureIntro. split; first set_solver. apply map_Forall_insert_2; done. }
+          rewrite decide_False //.
+          iStep 3 as (cnodes base base_descr _ Hbase_gen (Hbase_store_dom & Hbase_store_gen) nodes δs Hδs_nodup Hδs_gen Hδs) "Hcnodes_elem Hδs $". iSteps; iPureIntro.
+          { eapply Forall_impl; first done. intros (r' & (g' & v')) H.
+            destruct (decide (r = r')) as [<- | Hr'].
+            - rewrite lookup_insert. naive_solver.
+            - rewrite lookup_insert_ne //.
+          } {
+            clear Hδs_gen. generalize dependent ς.
+            induction δs as [| (r' & (g' & v')) δs IH] using rev_ind.
+            all: intros ς Hς_dom Hς_gen Hς_lookup Hδs.
+            - exfalso.
+              rewrite deltas_apply_nil in Hδs.
+              rewrite -Hδs store_on_lookup in Hς_lookup.
+              destruct Hς_lookup as [Hbase_store_lookup |]; last naive_solver.
+              opose proof* (map_Forall_lookup_1 _ base_descr.2); [done.. |].
+              naive_solver lia.
+            - rewrite deltas_apply_snoc /=.
+              destruct (decide (r = r')) as [<- | Hr'].
+              + rewrite deltas_apply_snoc /= in Hδs.
+                rewrite insert_insert //.
+              + rewrite insert_commute //.
+                apply IH; simpl.
+                * rewrite fmap_app NoDup_app in Hδs_nodup. naive_solver.
+                * rewrite dom_insert union_subseteq singleton_subseteq_l.
+                  split; last done.
+                  apply (f_equal dom) in Hδs.
+                  rewrite store_on_dom' // store_on_dom in Hδs.
+                  rewrite Hδs deltas_apply_dom. set_solver.
+                * apply map_Forall_insert_2; last done.
+                  trans base_descr.1; last lia.
+                  assert (store_on σ0 base_descr.2 !! r' = Some (g', v')) as [Hbase_store_lookup | (_ & ? & _)]%store_on_lookup; last lia.
+                  { rewrite Hδs.
+                    apply store_on_lookup', deltas_apply_lookup; first done.
+                    set_solver.
+                  }
+                  eapply map_Forall_lookup_1 in Hbase_store_gen; done.
+                * rewrite /store_on -insert_union_l lookup_insert_ne //.
+                * rewrite deltas_apply_snoc // in Hδs.
+          }
+        + rewrite bool_decide_eq_false_2; first naive_solver. wp_pures.
+          wp_alloc root' as "Hroot'". do 2 wp_load. do 4 wp_store.
+          iDestruct ("Hς" $! (g, v) with "[$Hr_gen $Hr_value]") as "Hς".
+          iApply "HΦ".
+          iExists l, γ, g, root', (<[r := (g, v)]> ς). iFrame "#∗". iStep.
+          iSplitR. { rewrite fmap_insert //. }
+          iSplitL "Hς". { rewrite insert_union_l //. }
+          iSplitR. { iPureIntro. split; first set_solver. apply map_Forall_insert_2; done. }
+          rewrite decide_False //.
+          iStep 3 as (cnodes base base_descr _ Hbase_gen (Hbase_store_dom & Hbase_store_gen) nodes δs Hδs_nodup Hδs_gen Hδs) "Hcnodes_elem Hδs $". iStep 2.
+          assert (r ∉ δs.*1) as Hr_notin_δs.
+          { intros (i & ((? & data) & -> & Hδs_lookup)%list_lookup_fmap_inv)%elem_of_list_lookup.
+            opose proof* Forall_lookup_1 as H; [done.. |].
+            apply store_on_lookup in Hς_lookup. naive_solver.
+          }
+          assert (store_on σ0 base_descr.2 !! r = Some (g_r, w)) as Hbase_store_lookup.
+          { rewrite Hδs store_on_lookup deltas_apply_lookup_ne //.
+            rewrite store_on_lookup // in Hς_lookup.
+          }
+          iExists (nodes ++ [root']), (δs ++ [(r, (g_r, w))]). iSteps; [iPureIntro.. |].
+          { rewrite fmap_app NoDup_app. split_and!; first done.
+            - set_solver.
+            - apply NoDup_singleton.
+          } {
+            rewrite Forall_app Forall_singleton. split.
+            - rewrite Forall_forall => δ Hδ. rewrite lookup_insert_ne.
+              { rewrite elem_of_list_fmap in Hr_notin_δs. naive_solver. }
+              rewrite Forall_forall in Hδs_gen. naive_solver.
+            - rewrite lookup_insert. naive_solver.
+          } {
+            rewrite deltas_apply_snoc insert_insert -deltas_apply_snoc'.
+            rewrite (deltas_apply_permutation ((r, (g_r, w)) :: δs)).
+            { rewrite fmap_app NoDup_app. split_and!; first done.
+              - set_solver.
+              - apply NoDup_singleton.
+            }
+            { solve_Permutation. }
+            rewrite deltas_apply_cons store_on_insert -Hδs insert_id //.
+          } {
+            iApply (deltas_chain_snoc with "Hδs Hroot").
+          }
+    Qed.
+
+    Lemma store_capture_spec t σ0 σ :
+      {{{
+        store_model t σ0 σ
+      }}}
+        store_capture t
+      {{{ s,
+        RET s;
+        store_model t σ0 σ ∗
+        store_snapshot_model s t σ
+      }}}.
+    Proof.
+      iIntros "%Φ (%l & %γ & %g & %root & %ς & -> & -> & #Hmeta & Hl_gen & Hl_root & Hroot & Hς & (%Hς_dom & %Hς_gen) & Hmodel) HΦ".
+      wp_rec. wp_load. wp_store. wp_load. wp_pures.
+      iApply "HΦ".
+      case_decide as Hg; first subst.
+      - pose descr := (0, ς).
+        iMod (cnodes_insert root descr with "Hmodel") as "(Hcnodes_auth & #Hcnodes_elem)"; first done.
+        iSplitL; last iSteps.
+        iExists l, γ, 1, root, ς. iFrame "#∗". iStep 2. iSplitR.
+        { iPureIntro. split; first set_solver.
+          eapply map_Forall_impl; first done. naive_solver.
+        }
+        iStep. iExists root, descr. iSplitR.
+        { iPureIntro. rewrite lookup_insert //. }
+        iStep. iSplitL.
+        { iStep 2. iExists [], []. iSteps.
+          - rewrite NoDup_nil //.
+          - rewrite deltas_apply_nil //.
+        }
+        rewrite insert_empty delete_singleton.
+        iApply (big_sepM_empty with "[//]").
+      - iDestruct "Hmodel" as "(%cnodes & %base & %base_descr & Hcnodes_auth & %Hcnodes_lookup_base & %Hbase_gen & ((%Hbase_store_dom & %Hbase_store_gen) & #Hcnodes_elem_base & %nodes & %δs & %Hδs_nodup & %Hδs_gen & %Hδs & Hδs) & Hcnodes)".
+        destruct δs as [| δ δs].
+        + iDestruct (deltas_chain_nil_inv with "Hδs") as %(-> & <-).
+          iSplitL; iSteps.
+          { iPureIntro. eapply map_Forall_impl; first done. naive_solver lia. }
+          rewrite decide_False; first lia.
+          iSteps. iExists []. iSteps.
+        + iAssert ⌜cnodes !! root = None⌝%I as %Hcnodes_lookup_root.
+          { destruct (decide (root = base)) as [-> | Hcase].
+            - iDestruct (deltas_chain_cons_inv with "Hδs") as "(%node & %nodes' & -> & Hbase & _)".
+              iDestruct (pointsto_ne with "Hroot Hbase") as %?. done.
+            - rewrite -eq_None_ne_Some. iIntros "%descr %Hcnodes_lookup".
+              iDestruct (big_sepM_lookup with "Hcnodes") as "(%cnode' & %descr' & _ & _ & _ & %nodes' & %δs' & _ & %Hδs'_length & _ & Hδs')".
+              { rewrite lookup_delete_Some //. }
+              destruct δs' as [| δ' δs']; first naive_solver lia.
+              iDestruct (deltas_chain_cons_inv with "Hδs'") as "(%node & %nodes'' & -> & _Hroot & _)".
+              iDestruct (pointsto_ne with "Hroot _Hroot") as %?. done.
+          }
+          pose root_descr := (g, ς).
+          iMod (cnodes_insert root root_descr with "Hcnodes_auth") as "(Hcnodes_auth & #Hcnodes_elem_root)"; first done.
+          iSplitL; last iSteps.
+          iExists l, γ, (S g), root, ς. iFrame "#∗". iSteps as (_ | _) "" | "".
+          { iPureIntro. eapply map_Forall_impl; first done. naive_solver. }
+          iExists root, root_descr. iSplitR.
+          { rewrite lookup_insert //. }
+          iStep. iSplitR.
+          { iStep 2. iExists [], []. iSteps; iPureIntro.
+            - rewrite NoDup_nil //.
+            - rewrite deltas_apply_nil //.
+          }
+        rewrite delete_insert //. iApply big_sepM_delete; first done.
+        iSteps. iExists root, root_descr. iSteps.
+        { iPureIntro. rewrite lookup_insert //. }
+        iApply (big_sepM_impl with "Hcnodes"). iIntros "!> !> %cnode %descr %Hcnodes_lookup_cnode (%cnode' & %descr' & %Hcnodes_lookup_cnode' & ((%Hcnode_store_dom & %Hcnode_store_gen) & #Hcnodes_elem_cnode & %nodes' & %δs' & %Hδs'_nodup & %Hδs'_length & %Hδs' & Hδs'))".
+        iSteps. iExists cnode', descr'. iSteps. iPureIntro.
+        rewrite lookup_insert_ne //. congruence.
+    Qed.
+
+    Lemma store_restore_spec t σ0 σ s σ' :
+      {{{
+        store_model t σ0 σ ∗
+        store_snapshot_model s t σ'
+      }}}
+        store_restore t s
+      {{{
+        RET ();
+        store_model t σ0 σ'
+      }}}.
+    Proof.
+    Admitted.
+  End store_G.
+
+  #[global] Opaque store_model.
+  #[global] Opaque store_snapshot_model.
+End raw.
+
+#[global] Opaque store_create.
+#[global] Opaque store_ref.
+#[global] Opaque store_get.
+#[global] Opaque store_set.
+#[global] Opaque store_capture.
+#[global] Opaque store_restore.
 
 Class StoreG Σ `{zebre_G : !ZebreG Σ} := {
-  #[local] store_G_nodes_G :: ghost_mapG Σ loc descriptor ;
+  #[local] store_G_raw_G :: raw.StoreG Σ ;
+  #[local] store_G_support_G :: MonoMapG Σ loc val ;
 }.
 
 Definition store_Σ := #[
-  ghost_mapΣ loc descriptor
+  raw.store_Σ ;
+  mono_map_Σ loc val
 ].
 Lemma subG_store_Σ Σ `{zebre_G : !ZebreG Σ} :
   subG store_Σ Σ →
@@ -169,98 +741,31 @@ Qed.
 Section store_G.
   Context `{store_G : StoreG Σ}.
 
-  #[local] Definition store_on σ0 ς :=
-    ς ∪ (pair 0 <$> σ0).
-  #[local] Definition store_generation g ς :=
-    map_Forall (λ r data, data.1 ≤ g) ς.
-
-  #[local] Definition delta : Set :=
-    loc * (generation * val).
-  Implicit Types δ : delta.
-  Implicit Types δs : list delta.
-
-  #[local] Definition delta_apply δs ς :=
-    list_to_map δs ∪ ς.
-  #[local] Fixpoint delta_chain node nodes δs dst : iProp Σ :=
-    match nodes, δs with
-    | [], [] =>
-        ⌜node = dst⌝
-    | node' :: nodes, δ :: δs =>
-        node ↦ ’Diff{ #δ.1, #δ.2.1, δ.2.2, #node' } ∗
-        delta_chain node' nodes δs dst
-    | _, _ =>
-        False
-    end.
-
-  #[local] Definition cnodes_auth γ cnodes :=
-    ghost_map_auth γ 1 cnodes.
-  #[local] Definition cnodes_pointsto γ cnode descr :=
-    ghost_map_elem γ cnode (DfracOwn 1) descr.
-  #[local] Definition cnodes_elem γ cnode descr :=
-    ghost_map_elem γ cnode DfracDiscarded descr.
-
-  #[local] Definition cnode_model γ σ0 cnode descr node ς : iProp Σ :=
-    ⌜dom descr.2 ⊆ dom σ0⌝ ∗
-    ⌜store_generation descr.1 descr.2⌝ ∗
-    cnodes_elem γ cnode descr ∗
-    ( ∃ nodes δs,
-      ⌜store_on σ0 descr.2 = store_on σ0 $ delta_apply δs ς⌝ ∗
-      delta_chain cnode nodes δs node
-    ).
-  Definition store_model t σ0 σ : iProp Σ :=
-    ∃ l γ g root ς,
+  Definition store_model t σ : iProp Σ :=
+    ∃ l γ σ0 ς,
     ⌜t = #l⌝ ∗
-    ⌜σ = snd <$> ς⌝ ∗
-    meta l nroot γ ∗
-    l.[gen] ↦ #g ∗
-    l.[root] ↦ #root ∗
-    root ↦ §Root ∗
-    ( [∗ map] r ↦ data ∈ store_on σ0 ς,
-      r.[ref_gen] ↦ #data.1 ∗
-      r.[ref_value] ↦ data.2
-    ) ∗
-    ⌜store_generation g ς⌝ ∗
-    if g is 0 then
-      cnodes_pointsto γ root (0, ς)
-    else
-      ∃ cnodes base base_descr,
-      cnodes_auth γ cnodes ∗
-      (* base cnode *)
-      ⌜cnodes !! base = Some base_descr⌝ ∗
-      ⌜base_descr.1 < g⌝ ∗
-      cnode_model γ σ0 base base_descr root ς ∗
-      (* other cnodes *)
-      ( [∗ map] cnode ↦ descr ∈ delete base cnodes,
-        ∃ cnode' descr',
-        ⌜cnodes !! cnode' = Some descr'⌝ ∗
-        cnode_model γ σ0 cnode descr cnode' descr'.2
-      ).
+    ⌜σ ⊆ ς ∪ σ0⌝ ∗
+    meta l (nroot.@"user") γ ∗
+    mono_map_auth γ σ0 ∗
+    raw.store_model t σ0 ς.
 
   Definition store_snapshot_model s t σ : iProp Σ :=
-    ∃ l γ g node descr,
-    ⌜t = #l ∧ s = (t, #g, #node)%V⌝ ∗
-    meta l nroot γ ∗
-    cnodes_elem γ node descr ∗
-    ⌜descr.1 ≤ g⌝.
+    ∃ l γ σ0 ς,
+    ⌜t = #l⌝ ∗
+    ⌜σ ⊆ ς ∪ σ0⌝ ∗
+    meta l (nroot.@"user") γ ∗
+    mono_map_lb γ σ0 ∗
+    raw.store_snapshot_model s t ς.
 
-  #[global] Instance store_model_timeless t σ0 σ :
-    Timeless (store_model t σ0 σ).
-  Proof.
-  Abort.
+  (* #[global] Instance store_model_timeless t σ : *)
+  (*   Timeless (store_model t σ). *)
+  (* Proof. *)
+  (*   apply _. *)
+  (* Qed. *)
   #[global] Instance store_snapshot_persistent s t σ :
     Persistent (store_snapshot_model s t σ).
   Proof.
     apply _.
-  Qed.
-
-  #[local] Definition cnodes_alloc root :
-    ⊢ |==>
-      ∃ γ,
-      cnodes_auth γ {[root := (0, ∅)]} ∗
-      cnodes_pointsto γ root (0, ∅).
-  Proof.
-    iMod ghost_map_alloc as "(%γ & Hcnodes_auth & Hcnodes_pointsto)".
-    iSteps. rewrite big_sepM_singleton. iSteps.
   Qed.
 
   Lemma store_create_spec :
@@ -268,91 +773,116 @@ Section store_G.
       store_create ()
     {{{ t,
       RET t;
-      store_model t ∅ ∅
+      store_model t ∅
     }}}.
   Proof.
     iIntros "%Φ _ HΦ".
-    wp_rec.
-    wp_alloc root as "Hroot".
-    wp_record l as "Hmeta" "(Hl_gen & Hl_root & _)".
-    iMod (cnodes_alloc root) as "(%γ & Hcnodes_auth & Hcnodes_pointsto)".
+    iApply wp_fupd.
+    wp_apply (raw.store_create_spec with "[//]") as (t) "((%l & -> & Hmeta) & Ht)".
+    iMod mono_map_alloc as "(%γ & Hauth)".
     iMod (meta_set with "Hmeta") as "Hmeta"; first done.
-    iApply "HΦ".
-    iExists l, γ, 0, root, ∅. iFrame. rewrite big_sepM_empty. iSteps.
+    iSteps. iExists ∅, ∅. iSteps.
   Qed.
 
-  Lemma store_ref_spec t σ0 σ v :
+  Lemma store_ref_spec t σ v :
     {{{
-      store_model t σ0 σ
+      store_model t σ
     }}}
       store_ref t v
     {{{ r,
       RET #r;
-      ⌜σ0 !! r = None⌝ ∗
-      store_model t (<[r := v]> σ0) σ
+      ⌜σ !! r = None⌝ ∗
+      store_model t (<[r := v]> σ)
     }}}.
   Proof.
-  Abort.
+    iIntros "%Φ (%l & %γ & %σ0 & %ς & -> & %Hσ & #Hmeta & Hauth & Ht) HΦ".
+    iDestruct (raw.store_model_valid with "Ht") as %Hς_dom.
+    iApply wp_fupd.
+    wp_apply (raw.store_ref_spec with "Ht") as (r) "(%Hσ0_lookup & Ht)".
+    assert (ς !! r = None) as Hς_lookup.
+    { rewrite -!not_elem_of_dom in Hσ0_lookup |- *. set_solver. }
+    assert (σ !! r = None) as Hσ_lookup.
+    { eapply lookup_weaken_None; last done. apply lookup_union_None_2; done. }
+    iMod (mono_map_insert with "Hauth") as "Hauth"; first done.
+    iApply "HΦ".
+    iStep. iExists l, γ, (<[r := v]> σ0), ς. iSteps. iPureIntro.
+    rewrite -insert_union_r //. apply insert_mono. done.
+  Qed.
 
-  Lemma store_get_spec {t σ0 σ r} v :
-    (σ ∪ σ0) !! r = Some v →
+  Lemma store_get_spec {t σ r} v :
+    σ !! r = Some v →
     {{{
-      store_model t σ0 σ
+      store_model t σ
     }}}
       store_get t #r
     {{{
       RET v;
-      store_model t σ0 σ
+      store_model t σ
     }}}.
   Proof.
-  Abort.
+    iIntros "%Hσ_lookup %Φ (%l & %γ & %σ0 & %ς & -> & %Hσ & #Hmeta & Hauth & Ht) HΦ".
+    wp_apply (raw.store_get_spec with "Ht") as "Ht".
+    { eapply lookup_weaken; done. }
+    iSteps.
+  Qed.
 
-  Lemma store_set_spec t σ0 σ r v :
-    r ∈ dom σ0 →
+  Lemma store_set_spec t σ r v :
+    r ∈ dom σ →
     {{{
-      store_model t σ0 σ
+      store_model t σ
     }}}
       store_set t #r v
     {{{
       RET ();
-      store_model t σ0 (<[r := v]> σ)
+      store_model t (<[r := v]> σ)
     }}}.
   Proof.
-  Abort.
+    iIntros "%Hr %Φ (%l & %γ & %σ0 & %ς & -> & %Hσ & #Hmeta & Hauth & Ht) HΦ".
+    iDestruct (raw.store_model_valid with "Ht") as %Hς_dom.
+    wp_apply (raw.store_set_spec with "Ht") as "Ht".
+    { apply subseteq_dom in Hσ. set_solver. }
+    iApply "HΦ".
+    iExists l, γ, σ0, (<[r := v]> ς). iSteps. iPureIntro.
+    rewrite -insert_union_l. apply insert_mono. done.
+  Qed.
 
-  Lemma store_capture_spec t σ0 σ :
+  Lemma store_capture_spec t σ :
     {{{
-      store_model t σ0 σ
+      store_model t σ
     }}}
       store_capture t
     {{{ s,
       RET s;
-      store_model t σ0 σ ∗
+      store_model t σ ∗
       store_snapshot_model s t σ
     }}}.
   Proof.
-  Abort.
+    iIntros "%Φ (%l & %γ & %σ0 & %ς & -> & %Hσ & #Hmeta & Hauth & Ht) HΦ".
+    iDestruct (mono_map_lb_get with "Hauth") as "#Hlb".
+    wp_apply (raw.store_capture_spec with "Ht") as (s) "(Ht & Hs)".
+    iSteps.
+  Qed.
 
-  Lemma store_restore_spec t σ0 σ s σ' :
+  Lemma store_restore_spec t σ s σ' :
     {{{
-      store_model t σ0 σ ∗
+      store_model t σ ∗
       store_snapshot_model s t σ'
     }}}
       store_restore t s
     {{{
       RET ();
-      store_model t σ0 σ'
+      store_model t σ'
     }}}.
   Proof.
-  Abort.
+    iIntros "%Φ ((%l & %γ & %σ0 & %ς & -> & %Hσ & #Hmeta & Hauth & Ht) & (%_l & %_γ & %σ0' & %ς' & %Heq & %Hσ' & _Hmeta & #Hlb & Hs)) HΦ". injection Heq as <-.
+    iDestruct (meta_agree with "Hmeta _Hmeta") as %<-. iClear "_Hmeta".
+    wp_apply (raw.store_restore_spec with "[$Ht $Hs]") as "Ht".
+    iDestruct (mono_map_valid with "Hauth Hlb") as %Hσ0'.
+    iApply "HΦ".
+    iExists l, γ, σ0, ς'. iSteps. iPureIntro.
+    trans (ς' ∪ σ0'); first done. apply map_union_mono_l. done.
+  Qed.
 End store_G.
-
-#[global] Opaque store_create.
-#[global] Opaque store_ref.
-#[global] Opaque store_get.
-#[global] Opaque store_set.
-#[global] Opaque store_capture.
-#[global] Opaque store_restore.
 
 #[global] Opaque store_model.
 #[global] Opaque store_snapshot_model.
