theories/iris/base_logic/lib/mono_map_.v
@@ -1,0 +1,66 @@
+From zebre Require Import
+  prelude.
+From zebre.iris.base_logic Require Export
+  lib.base.
+From zebre.iris Require Import
+  diaframe.
+From zebre Require Import
+  options.
+
+Class MonoMapG (Σ : gFunctors) (K V : Type) `{Countable K} := {
+}.
+
+Definition mono_map_Σ (K V : Type) `{Countable K} := #[
+].
+#[global] Instance subG_mono_map_Σ Σ K V `{Countable K} :
+  subG (mono_map_Σ K V) Σ →
+  MonoMapG Σ K V.
+Proof.
+Qed.
+
+Section mono_map_G.
+  Context `{mono_map_G : MonoMapG Σ K V}.
+
+  Implicit Types γ : gname.
+  Implicit Types m : gmap K V.
+
+  Definition mono_map_auth γ m : iProp Σ.
+  Proof. Admitted.
+  Definition mono_map_lb γ m : iProp Σ.
+  Proof. Admitted.
+
+  #[global] Instance mono_map_lb_persistent γ m :
+    Persistent (mono_map_lb γ m).
+  Proof.
+  Admitted.
+
+  Lemma mono_map_alloc m :
+    ⊢ |==>
+      ∃ γ,
+      mono_map_auth γ m.
+  Proof.
+  Admitted.
+
+  Lemma mono_map_insert {γ m} i v :
+    m !! i = None →
+    mono_map_auth γ m ⊢ |==>
+    mono_map_auth γ (<[i := v]> m).
+  Proof.
+  Admitted.
+
+  Lemma mono_map_lb_get γ m :
+    mono_map_auth γ m ⊢
+    mono_map_lb γ m.
+  Proof.
+  Admitted.
+
+  Lemma mono_map_valid γ m1 m2 :
+    mono_map_auth γ m1 -∗
+    mono_map_lb γ m2 -∗
+    ⌜m2 ⊆ m1⌝.
+  Proof.
+  Admitted.
+End mono_map_G.
+
+#[global] Opaque mono_map_auth.
+#[global] Opaque mono_map_lb.
